Authentication_Tests.v
@@ -1,0 +1,8 @@
+
+Require Import Strand_Spaces Strand_Library Message_Algebra Authentication_Tests_Library.
+
+Section TestComponent.
+Variable a t : msg.
+Variable n : node.
+
+End TestComponent.
